code/ecdsap256sha2/Hacl.Impl.P256.LowLevel.fst
@@ -36,6 +36,7 @@ val reduction_prime256_2prime256_with_carry_impl: cin: uint64 -> x: felem -> res
     (ensures fun h0 _ h1 -> 
       modifies (loc result) h0 h1 /\ 
       as_nat h1 result < prime /\ 
+      inField h1 result /\ 
       as_nat_elem1 h1 result = (as_nat h0 x + uint_v cin * pow2 256) % prime /\
       as_nat_elem h1 result = (as_nat h0 x + uint_v cin * pow2 256) % prime
     )  
